%-*-latex-*-
\tinysidebar{\debug{exercises/{introduction-to-group-theory-abelian-exponentiation/answer.tex}}}
First I'll prove the statement for positive integers:

Lemma A.
$(x * y)^n = x^n * y^n$ for $n \geq 0$.

I will prove Lemma A by induction.
Since
\[
(x * y)^0 = e
\]
and
\[
x^0 * y^0 = e * e = e
\]
the statement is true for $n = 0$.
Assume the statement is true for $n$.
We have
\begin{align*}
(x * y)^{n+1}
&= (x * y)^{n} * (x * y) & & \text{by definition of exponentiation}\\
&= (x^n * y^n) * (x * y) & & \text{by inductive hypothesis} \\
&= ((x^n * y^n) * x) * y & & \text{by associativity} \\
&= (x^n * (y^n * x)) * y & & \text{by associativity} \\
&= (x^n * (x * y^n)) * y & & \text{by abelian property} \\
&= ((x^n * x) * y^n) * y & & \text{by associativity} \\
&= (x^{n+1} * y^n) * y    & & \text{by definition of exponentiation}\\
&= x^{n+1} * (y^n * y)    & & \text{by associativity}\\
&= x^{n+1} * y^{n+1}       & & \text{by definition of exponentiation}
\end{align*}
Hence by induction
\[
(x * y)^n = x^n * y^n
\]
for $n \geq 0$.
Lemma A is proven.

Now I will prove the above formula for negative $n$:
\begin{align*}
(x * y)^n
&= ((x * y)^{-1})^{-n}            & & \text{by definition of exponentiation}\\
&= (y^{-1} * x^{-1})^{-n}          & & \text{by ??} \\
&= ((y^{-1})^{-n} * (x^{-1}))^{-n}  & & \text{by Lemma A} \\
&= (y^{n} * x^{n})                & & \text{by definition of exponentiation}\\
&= (x^{n} * y^{n})                & & \text{by abelian property}
\end{align*}
Therefore
\[
(x * y)^n = x^n * y^n
\]
for $n \in \Z$ and $n < 0$.

Hence altogether
\[
(x * y)^n = x^n * y^n
\]
for $n \in \Z$.
\qed
